WIP

theories/Eq/Eq.v
@@ -9,7 +9,7 @@
     Goal (cofix spin := Tau spin) = (cofix spin2 := Tau (Tau spin2)).
 ]]
     As an alternative, we define a weaker, coinductive notion of equivalence,
-    [eq_itree], which can be intuitively thought of as a form of extensional
+    [eqit], which can be intuitively thought of as a form of extensional
     equality. We shall rely extensively on setoid rewriting.
  *)
 
@@ -58,11 +58,13 @@ Proof. auto. Qed.
     instead encoding a form of productivity visibly in types.
  *)
 
-Section eq_itree.
+Coercion is_true : bool >-> Sortclass.
+
+Section eqit.
 
   (** Although the original motivation is to define an equivalence
       relation on [itree E R], we will generalize it into a
-      heterogeneous relation [eq_itree_] between [itree E R1] and
+      heterogeneous relation [eqit_] between [itree E R1] and
       [itree E R2], parameterized by a relation [RR] between [R1]
       and [R2].
 
@@ -73,74 +75,86 @@ Section eq_itree.
 
   (** We also need to do some gymnastics to work around the
       two-layered definition of [itree]. We first define a
-      relation transformer [eq_itreeF] as an indexed inductive type
+      relation transformer [eqitF] as an indexed inductive type
       on [itreeF], which is then composed with [observe] to obtain
-      a relation transformer on [itree] ([eq_itree_]).
+      a relation transformer on [itree] ([eqit_]).
 
       In short, this is necessitated by the fact that dependent
       pattern-matching is not allowed on [itree].
    *)
 
-  Inductive eq_itreeF (sim : itree E R1 -> itree E R2 -> Prop) :
+  Inductive eqitF (bl br: bool) (sim : itree E R1 -> itree E R2 -> Prop) :
     itree' E R1 -> itree' E R2 -> Prop :=
-  | EqRet : forall r1 r2, RR r1 r2 -> eq_itreeF sim (RetF r1) (RetF r2)
+  | EqRet : forall r1 r2, RR r1 r2 -> eqitF bl br sim (RetF r1) (RetF r2)
   | EqTau : forall m1 m2
-      (REL: sim m1 m2), eq_itreeF sim (TauF m1) (TauF m2)
+      (REL: sim m1 m2), eqitF bl br sim (TauF m1) (TauF m2)
   | EqVis : forall {u} (e : E u) k1 k2
       (REL: forall v, sim (k1 v) (k2 v)),
-      eq_itreeF sim (VisF e k1) (VisF e k2)
+      eqitF bl br sim (VisF e k1) (VisF e k2)
+  | EqTauL t1 ot2
+      (CHECK: bl)
+      (REL: eqitF bl br sim (observe t1) ot2):
+      eqitF bl br sim (TauF t1) ot2
+  | EqTauR ot1 t2
+      (CHECK: br)
+      (REL: eqitF bl br sim ot1 (observe t2)):
+      eqitF bl br sim ot1 (TauF t2)
   .
-  Hint Constructors eq_itreeF.
+  Hint Constructors eqitF.
 
-  Definition eq_itree_ (sim: itree E R1 -> itree E R2 -> Prop) :
+  Definition eqit_ bl br (sim: itree E R1 -> itree E R2 -> Prop) :
     itree E R1 -> itree E R2 -> Prop :=
-    fun t1 t2 => eq_itreeF sim (observe t1) (observe t2).
-  Hint Unfold eq_itree_.
+    fun t1 t2 => eqitF bl br sim (observe t1) (observe t2).
+  Hint Unfold eqit_.
 
-  (** [eq_itreeF] and [eq_itree_] are both monotone. *)
+  (** [eqitF] and [eqit_] are both monotone. *)
 
-  Lemma eq_itreeF_mono x0 x1 (r r' : itree E R1 -> itree E R2 -> Prop) :
+  Lemma eqitF_mono bl br x0 x1 (r r' : itree E R1 -> itree E R2 -> Prop) :
     forall
-      (IN: eq_itreeF r x0 x1)
+      (IN: eqitF bl br r x0 x1)
       (LE: forall x2 x3, r x2 x3 -> r' x2 x3 : Prop),
-        eq_itreeF r' x0 x1.
-  Proof. pmonauto. Qed.
+        eqitF bl br r' x0 x1.
+  Proof. intros. induction IN; eauto. Qed.
 
-  Lemma eq_itree__mono : monotone2 eq_itree_.
-  Proof. do 2 red. pmonauto. Qed.
+  Lemma eqit__mono bl br : monotone2 (eqit_ bl br).
+  Proof. do 2 red. intros. eapply eqitF_mono; eauto. Qed.
 
-  (** Strong bisimulation on itrees. If [eq_itree RR t1 t2],
+  Definition eqit bl br : itree E R1 -> itree E R2 -> Prop :=
+    gcpn2 (eqit_ bl br) bot2 bot2.
+
+  (** Strong bisimulation on itrees. If [eqit RR t1 t2],
       we say that [t1] and [t2] are (strongly) bisimilar. As hinted
       at above, bisimilarity can be intuitively thought of as
       equality. *)
-  Definition eq_itree : itree E R1 -> itree E R2 -> Prop :=
-    gcpn2 eq_itree_ bot2 bot2.
-
-  Lemma eq_itree_fold :
-    eq_itree <2= gcpn2 eq_itree_ bot2 bot2.
-  Proof. intros. apply PR. Qed.
-  Hint Resolve eq_itree_fold.
   
-End eq_itree.
+  Definition eq_itree := eqit false false.
+
+  Definition eutt := eqit true true.
+
+  Definition eutble := eqit false true.
+
+End eqit.
 
 (* begin hide *)
-Hint Constructors eq_itreeF.
-Hint Unfold eq_itree_.
-Hint Resolve eq_itree__mono : paco.
+Hint Constructors eqitF.
+Hint Unfold eqit_.
+Hint Resolve eqit__mono : paco.
+Hint Unfold eqit.
 Hint Unfold eq_itree.
-Hint Resolve eq_itree_fold.
+Hint Unfold eutt.
+Hint Unfold eutble.
 
-Ltac unfold_eq_itree :=
-  (try match goal with [|- eq_itree_ _ _ _ _ ] => red end);
-  (repeat match goal with [H: eq_itree_ _ _ _ _ |- _ ] => red in H end).
+Ltac unfold_eqit :=
+  (try match goal with [|- eqit_ _ _ _ _ _ _ ] => red end);
+  (repeat match goal with [H: eqit_ _ _ _ _ _ _ |- _ ] => red in H end).
 
-Lemma flip_eq_itree {E R1 R2} (RR : R1 -> R2 -> Prop) :
+Lemma flip_eqit {E R1 R2} (RR : R1 -> R2 -> Prop) bl br :
   forall (u : itree E R1) (v : itree E R2),
-    eq_itree RR u v -> eq_itree (flip RR) v u.
+    eqit RR bl br u v -> eqit (flip RR) br bl v u.
 Proof.
   gcofix self; gstep.
   intros u v euv. gunfold euv.
-  repeat red; destruct euv; eauto 10 with paco.
+  red in euv |- *. induction euv; eauto with paco.
 Qed.
 (* end hide *)
 
@@ -148,34 +162,46 @@ Delimit Scope eq_itree_scope with eq_itree.
 
 (** A notation of [eq_itree eq]. You can write [≅] using [[\cong]] in
     tex-mode *)
-Notation "t1 ≅ t2" := (eq_itree eq t1%itree t2%itree) (at level 70).
 
-Section eq_itree_h.
+Open Scope itree_scope.
+
+Infix "≅" := (eq_itree eq) (at level 70) : itree_scope.
+
+Infix "≈" := (eutt eq) (at level 70) : itree_scope.
+
+Infix "≲" := (eutble eq) (at level 70) : itree_scope.
+
+Section eqit_h.
 
 Context {E : Type -> Type} {R1 R2 : Type} (RR : R1 -> R2 -> Prop).
 
-(** [eq_itree] is a congruence for [itree] constructors. *)
+(** [eqit] is a congruence for [itree] constructors. *)
 
-Lemma eq_itree_Tau (t1 : itree E R1) (t2 : itree E R2) :
-  eq_itree RR (Tau t1) (Tau t2) <-> eq_itree RR t1 t2.
+Lemma eqit_Tau bl br (t1 : itree E R1) (t2 : itree E R2) :
+  eqit RR bl br (Tau t1) (Tau t2) <-> eqit RR bl br t1 t2.
 Proof.
   split; intros H.
-  - gunfold H; inversion H; eauto.
+  - gunfold H. red in H. simpl in *. gstep. red.
+    remember (TauF t1) as ot1. remember (TauF t2) as ot2.
+    hinduction H before RR; intros; subst; try inv Heqot1; try inv Heqot2; eauto.
+    + gunfold REL. eauto.
+    + inv H; eauto.
+    + inv H; eauto.
   - gstep. constructor; auto.
 Qed.
 
-Lemma eq_itree_Vis {U} (e : E U)
+Lemma eqit_Vis bl br {U} (e : E U)
       (k1 : U -> itree E R1) (k2 : U -> itree E R2) :
-      (forall u, eq_itree RR (k1 u) (k2 u))
-  <-> eq_itree RR (Vis e k1) (Vis e k2).
+      (forall u, eqit RR bl br (k1 u) (k2 u))
+  <-> eqit RR bl br (Vis e k1) (Vis e k2).
 Proof.
   split; intros H.
   - gstep. econstructor. eauto with paco. 
   - gunfold H. inversion H; auto_inj_pair2; subst; auto.
 Qed.
 
-Lemma eq_itree_Ret (r1 : R1) (r2 : R2) :
-  RR r1 r2 <-> @eq_itree E _ _ RR (Ret r1) (Ret r2).
+Lemma eqit_Ret bl br (r1 : R1) (r2 : R2) :
+  RR r1 r2 <-> @eqit E _ _ RR bl br (Ret r1) (Ret r2).
 Proof.
   split; intros H.
   - gstep. constructor; auto.
@@ -184,206 +210,223 @@ Qed.
 
 (** *** "Up-to" principles for coinduction. *)
 
-Inductive eq_trans_clo (r : itree E R1 -> itree E R2 -> Prop) :
-  itree E R1 -> itree E R2 -> Prop :=
-| eq_trans_clo_intro t1 t2 t3 t4
-      (EQVl: eq_itree eq t1 t2)
-      (EQVr: eq_itree eq t4 t3)
-      (RELATED: r t2 t3)
-  : eq_trans_clo r t1 t4
+Inductive eqit_trans_clo bl1 br1 bl2 br2 (r : itree E R1 -> itree E R2 -> Prop) : itree E R1 -> itree E R2 -> Prop :=
+| eqit_trans_clo_intro t1 t2 t1' t2'
+      (EQVl: eqit eq bl1 br1 t1' t1)
+      (EQVr: eqit eq bl2 br2 t2' t2)
+      (RELATED: r t1' t2')
+  : eqit_trans_clo bl1 br1 bl2 br2 r t1 t2
 .
-Hint Constructors eq_trans_clo.
+Hint Constructors eqit_trans_clo.
 
-Lemma eq_itree_clo_trans : eq_trans_clo <3= cpn2 (eq_itree_ RR).
+Lemma eqit_clo_trans (bl br br1 br2: bool)
+    (COND1: br1 -> bl) (COND2: br2 -> br):
+  eqit_trans_clo false br1 false br2 <3= cpn2 (eqit_ RR bl br).
 Proof.
   ucompat. econstructor; [pmonauto|].
   intros. dependent destruction PR.
-  gunfold EQVl. gunfold EQVr. unfold_eq_itree.
-  inversion EQVl;
-    inversion EQVr; clear EQVr;
-    inversion RELATED; clear RELATED;
-      subst; simpobs; try discriminate.
-
-  - inversion H0; inversion H3; auto.
-  - inversion H; inversion H3; subst; eauto with rclo.
-  - inversion H; inversion H3; subst; auto_inj_pair2; subst.
-    econstructor. intros. specialize (REL v). specialize (REL0 v).
-    eauto with rclo.
+  gunfold EQVl. gunfold EQVr. unfold_eqit.
+  hinduction RELATED before r; intros; clear t1' t2'.
+  - remember (RetF r1) as x.
+    hinduction EQVl before r; intros; subst; try inv Heqx; eauto.
+    remember (RetF r3) as y.
+    hinduction EQVr before r; intros; subst; try inv Heqy; eauto.
+  - remember (TauF m1) as x.
+    hinduction EQVl before r; intros; subst; try inv Heqx; try inv CHECK; eauto.
+    remember (TauF m3) as y.
+    hinduction EQVr before r; intros; subst; try inv Heqy; try inv CHECK; eauto.
+    econstructor. apply rclo2_clo. econstructor; cycle -1.
+    + apply rclo2_base. eauto.
+    + eauto.
+    + eauto.
+  - remember (VisF e k1) as x.
+    hinduction EQVl before r; intros; subst; try dependent destruction Heqx; try inv CHECK; eauto.
+    remember (VisF e0 k3) as y.
+    hinduction EQVr before r; intros; subst; try dependent destruction Heqy; try inv CHECK; eauto.
+    econstructor. intros. apply rclo2_clo. econstructor; cycle -1.
+    + apply rclo2_base. eauto.
+    + eauto.
+    + eauto.
+  - remember (TauF t1) as x.
+    hinduction EQVl before r; intros; subst; try inv Heqx; try inv CHECK; eauto.
+    gunfold REL. econstructor; eauto.
+  - remember (TauF t2) as y.
+    hinduction EQVr before r; intros; subst; try inv Heqy; try inv CHECK; eauto.
+    gunfold REL. econstructor; eauto.
 Qed.
 
-Inductive eq_bind_clo (r : itree E R1 -> itree E R2 -> Prop) :
+Inductive eqit_bind_clo bl br (r : itree E R1 -> itree E R2 -> Prop) :
   itree E R1 -> itree E R2 -> Prop :=
 | pbc_intro_h U1 U2 (RU : U1 -> U2 -> Prop) t1 t2 k1 k2
-      (EQV: eq_itree RU t1 t2)
+      (EQV: eqit RU bl br t1 t2)
       (REL: forall u1 u2, RU u1 u2 -> r (k1 u1) (k2 u2))
-  : eq_bind_clo r (ITree.bind t1 k1) (ITree.bind t2 k2)
+  : eqit_bind_clo bl br r (ITree.bind t1 k1) (ITree.bind t2 k2)
 .
-Hint Constructors eq_bind_clo.
+Hint Constructors eqit_bind_clo.
 
-Lemma eq_itree_clo_bind : eq_bind_clo <3= cpn2 (eq_itree_ RR).
+Lemma eqit_clo_bind bl br: eqit_bind_clo bl br <3= cpn2 (eqit_ RR bl br).
 Proof.
   ucompat. econstructor; [pmonauto|].
   intros. dependent destruction PR.
-  gunfold EQV. unfold_eq_itree.
-  rewrite !unfold_bind; destruct EQV; simpobs.
-  - eapply eq_itreeF_mono; [eapply REL |]; eauto with rclo.
+  gunfold EQV. unfold_eqit. rewrite !unfold_bind. 
+  hinduction EQV before r; intros.
+  - eapply eqitF_mono; [eapply REL |]; eauto with rclo.
   - simpl. eauto 8 with rclo.
   - econstructor.
-    intros x. specialize (REL0 x). eauto 7 with rclo.
+    intros x. specialize (REL x). eauto 7 with rclo.
+  - econstructor; eauto. rewrite unfold_bind; eauto.
+  - econstructor; eauto. rewrite unfold_bind; eauto.
 Qed.
 
-End eq_itree_h.
+End eqit_h.
 
-Arguments eq_itree_clo_trans : clear implicits.
-Arguments eq_itree_clo_bind : clear implicits.
+Arguments eqit_clo_trans : clear implicits.
+Arguments eqit_clo_bind : clear implicits.
 
-Hint Constructors eq_trans_clo.
-Hint Constructors eq_bind_clo.
+Hint Constructors eqit_trans_clo.
+Hint Constructors eqit_bind_clo.
 
 (** *** One-sided inversion *)
 
-Lemma eq_itree_ret_inv1 {E R} (t : itree E R) r :
+Lemma eqit_ret_inv1 {E R} (t : itree E R) r :
   t ≅ (Ret r) -> observe t = RetF r.
 Proof.
-  intros; gunfold H; inversion H; subst; auto.
+  intros; gunfold H; inv H; try inv CHECK; eauto.
 Qed.
 
-Lemma eq_itree_vis_inv1 {E R U} (t : itree E R) (e : E U) (k : U -> _) :
+Lemma eqit_vis_inv1 {E R U} (t : itree E R) (e : E U) (k : U -> _) :
   t ≅ Vis e k -> exists k', observe t = VisF e k' /\ forall u, k' u ≅ k u.
 Proof.
-  intros; gunfold H; inversion H; subst; auto_inj_pair2; subst; eauto.
+  intros; gunfold H; inv H; auto_inj_pair2; subst; try inv CHECK; eauto.
 Qed.
 
-Lemma eq_itree_tau_inv1 {E R} (t t' : itree E R) :
+Lemma eqit_tau_inv1 {E R} (t t' : itree E R) :
   t ≅ Tau t' -> exists t0, observe t = TauF t0 /\ t0 ≅ t'.
 Proof.
-  intros; gunfold H; inversion H; eauto.
+  intros; gunfold H; inv H; try inv CHECK; eauto.
 Qed.
 
 (** ** Properties of relations *)
 
 (** Instances stating that we have equivalence relations. *)
 
-Section eq_itree_eq.
+Section eqit_eq.
 
-  (** *** Properties of relation transformers. *)
+(** *** Properties of relation transformers. *)
 
-  Context {E : Type -> Type} {R : Type}.
+Context {E : Type -> Type} {R : Type}.
 
-  Local Notation eq_itree := (@eq_itree E R R eq).
+Local Notation eqit := (@eqit E R R eq).
 
-  Global Instance Reflexive_eq_itreeF (sim : itree E R -> itree E R -> Prop)
-  : Reflexive sim -> Reflexive (eq_itreeF eq sim).
-  Proof.
-    red. destruct x; constructor; eauto.
-  Qed.
+Global Instance Reflexive_eqitF bl br (sim : itree E R -> itree E R -> Prop)
+: Reflexive sim -> Reflexive (eqitF eq bl br sim).
+Proof.
+  red. destruct x; constructor; eauto.
+Qed.
 
-  Global Instance Symmetric_eq_itreeF (sim : itree E R -> itree E R -> Prop)
-  : Symmetric sim -> Symmetric (eq_itreeF eq sim).
-  Proof.
-    red. inversion 2; constructor; eauto.
-  Qed.
+Global Instance Symmetric_eqitF b (sim : itree E R -> itree E R -> Prop)
+: Symmetric sim -> Symmetric (eqitF eq b b sim).
+Proof.
+  red. induction 2; constructor; subst; eauto.
+Qed.
 
-  Global Instance Transitive_eq_itreeF (sim : itree E R -> itree E R -> Prop)
-  : Transitive sim -> Transitive (eq_itreeF eq sim).
-  Proof.
-    red. inversion 2; inversion 1; subst; repeat auto_inj_pair2; subst; constructor; eauto.
-  Qed.
+Global Instance Reflexive_eqit_ bl br (sim : itree E R -> itree E R -> Prop)
+: Reflexive sim -> Reflexive (eqit_ eq bl br sim).
+Proof. repeat red. reflexivity. Qed.
 
-  Global Instance Reflexive_eq_itree_ (sim : itree E R -> itree E R -> Prop)
-  : Reflexive sim -> Reflexive (eq_itree_ eq sim).
-  Proof. repeat red. reflexivity. Qed.
+Global Instance Symmetric_eqit_ b (sim : itree E R -> itree E R -> Prop)
+: Symmetric sim -> Symmetric (eqit_ eq b b sim).
+Proof. repeat red; symmetry; auto. Qed.
 
-  Global Instance Symmetric_eq_itree_ (sim : itree E R -> itree E R -> Prop)
-  : Symmetric sim -> Symmetric (eq_itree_ eq sim).
-  Proof. repeat red; symmetry; auto. Qed.
+(** *** [eqit] is an equivalence relation *)
 
-  Global Instance Transitive_eq_itree_ (sim : itree E R -> itree E R -> Prop)
-  : Transitive sim -> Transitive (eq_itree_ eq sim).
-  Proof. repeat red; etransitivity; eauto. Qed.
-
-(** *** [eq_itree] is an equivalence relation *)
-
-Global Instance Reflexive_eq_itree_gen (r rg: itree E R -> itree E R -> Prop) :
-  Reflexive (gcpn2 (eq_itree_ eq) r rg).
+Global Instance Reflexive_eqit_gen bl br (r rg: itree E R -> itree E R -> Prop) :
+  Reflexive (gcpn2 (eqit_ eq bl br) r rg).
 Proof.
   repeat intro. eapply gcpn2_mon_bot; eauto with paco.
   revert x. gcofix CIH; gstep; intros.
   repeat red. destruct (observe x); eauto with paco.
 Qed.
 
-Global Instance Reflexive_eq_itree : Reflexive eq_itree.
+Global Instance Reflexive_eqit bl br : Reflexive (eqit bl br).
 Proof.
-  apply Reflexive_eq_itree_gen.
+  apply Reflexive_eqit_gen.
 Qed.
 
-Global Instance Symmetric_eq_itree : Symmetric eq_itree.
+Global Instance Symmetric_eqit b : Symmetric (eqit b b).
 Proof.
   gcofix CIH; gstep; intros.
-  repeat red. gunfold H0. inv H0; eauto with paco.
+  repeat red. gunfold H0. red in H0.
+  induction H0; eauto with paco.
 Qed.
 
-Global Instance Transitive_eq_itree : Transitive eq_itree.
+Global Instance Transitive_eqit (br: bool) : Transitive (eqit false br).
 Proof.
-  gcofix CIH; gstep. intros.
-  repeat red.
-  gunfold H0; repeat red in H0.
-  gunfold H1; repeat red in H1.
-  destruct H0; inversion H1; subst; eauto.
-  - eauto with paco.
-  - auto_inj_pair2; subst.
-    subst; econstructor. intros. specialize (REL v). specialize (REL0 v). eauto with paco.
+  repeat intro.
+  gclo eqit_clo_trans; eauto.
+  econstructor; eauto.
+  reflexivity.
 Qed.
 
-Global Instance Equivalence_eq_itree : Equivalence eq_itree.
+Global Instance Equivalence_eqit : Equivalence (eqit false false).
 Proof.
   constructor; try typeclasses eauto.
 Qed.
 
 (** *** Congruence properties *)
 
-Global Instance eq_itree_observe :
-  Proper (eq_itree ==> going eq_itree) (@observe E R).
+Global Instance eqit_observe bl br:
+  Proper (eqit bl br ==> going (eqit bl br)) (@observe E R).
 Proof.
-  constructor; gunfold H. gstep. eapply eq_itreeF_mono; eauto.
+  constructor; gunfold H. gstep. eapply eqitF_mono; eauto.
 Qed.
 
-Global Instance eq_itree_tauF :
-  Proper (eq_itree ==> going eq_itree) (@TauF E R _).
+Global Instance eqit_tauF bl br:
+  Proper (eqit bl br ==> going (eqit bl br)) (@TauF E R _).
 Proof.
   constructor; gstep. econstructor. eauto.
 Qed.
 
-Global Instance eq_itree_VisF {u} (e: E u) :
-  Proper (pointwise_relation _ eq_itree ==> going eq_itree) (VisF e).
+Global Instance eqit_VisF bl br {u} (e: E u) :
+  Proper (pointwise_relation _ (eqit bl br) ==> going (eqit bl br)) (VisF e).
 Proof.
   constructor; red in H. gstep; econstructor. apply H.
 Qed.
 
-  Global Instance observing_eq_itree_eq_ (r: itree E R -> itree E R -> Prop) `{Reflexive _ r} :
-    subrelation (observing eq) (eq_itree_ eq r).
-  Proof.
-    repeat red; intros x _ [[]]; destruct observe; auto.
-  Qed.
-  
-  Global Instance observing_eq_itree_eq :
-    subrelation (observing eq) eq_itree.
-  Proof.
-    repeat red; intros; gstep. apply observing_eq_itree_eq_; auto.
-    apply Reflexive_eq_itree.
-  Qed.
+Global Instance observing_sub_eqit l r :
+  subrelation (observing eq) (eqit l r).
+Proof.
+  repeat red; intros; gstep. destruct H.
+  red. rewrite H. apply reflexivity.
+Qed.
+
+Global Instance eq_sub_eqit l r:
+  subrelation (eqit false false) (eqit l r).
+Proof.
+  gcofix CIH. intros.
+  gunfold H0. gstep. red in H0 |- *.
+  hinduction H0 before CIH; subst; econstructor; eauto with paco; inv CHECK.
+Qed.  
+
+Global Instance eqit_sub_eutt l r:
+  subrelation (eqit l r) (eqit true true).
+Proof.
+  gcofix CIH. intros.
+  gunfold H0. gstep. red in H0 |- *.
+  hinduction H0 before CIH; subst; econstructor; eauto with paco.
+Qed.  
 
 (** ** Eta-expansion *)
 
 Lemma itree_eta (t : itree E R) : t ≅ go (observe t).
-Proof. apply observing_eq_itree_eq. econstructor. reflexivity. Qed.
+Proof. apply observing_sub_eqit. econstructor. reflexivity. Qed.
 
 Lemma itree_eta' (ot : itree' E R) : ot = observe (go ot).
 Proof. reflexivity. Qed.
 
-End eq_itree_eq.
+End eqit_eq.
 
-Hint Resolve Reflexive_eq_itree Reflexive_eq_itree_gen : reflexivity.
+Hint Resolve Reflexive_eqit Reflexive_eqit_gen : reflexivity.
 
 (** ** Equations for core combinators *)
 
@@ -414,51 +457,76 @@ Proof.
   reflexivity.
 Qed.
 
-Lemma eq_itree_bind' {E R1 R2 S1 S2} (RR : R1 -> R2 -> Prop)
+Lemma eqit_bind' {E R1 R2 S1 S2} (RR : R1 -> R2 -> Prop) bl br
       (RS : S1 -> S2 -> Prop)
       t1 t2 k1 k2 :
-  eq_itree RR t1 t2 ->
-  (forall r1 r2, RR r1 r2 -> eq_itree RS (k1 r1) (k2 r2)) ->
-  @eq_itree E _ _ RS (ITree.bind t1 k1) (ITree.bind t2 k2).
+  eqit RR bl br t1 t2 ->
+  (forall r1 r2, RR r1 r2 -> eqit RS bl br (k1 r1) (k2 r2)) ->
+  @eqit E _ _ RS bl br (ITree.bind t1 k1) (ITree.bind t2 k2).
 Proof.
-  gclo eq_itree_clo_bind. eauto 7 with paco.
+  intros. gclo eqit_clo_bind. econstructor; eauto with paco.
 Qed.
 
-Instance eq_itree_bind {E R S} :
-  Proper (pointwise_relation _ (eq_itree eq) ==>
-          eq_itree eq ==>
-          eq_itree eq) (@ITree.bind' E R S).
+Instance eqit_bind {E R S} bl br :
+  Proper (pointwise_relation _ (eqit eq bl br) ==>
+          eqit eq bl br ==>
+          eqit eq bl br) (@ITree.bind' E R S).
 Proof.
-  repeat intro; eapply eq_itree_bind'; eauto.
+  repeat intro; eapply eqit_bind'; eauto.
   intros; subst; auto.
 Qed.
 
-Lemma eq_itree_map {E R1 R2 S1 S2} (RR : R1 -> R2 -> Prop)
+Instance eqit_bind_ {E R S} bl br :
+  Proper (pointwise_relation _ (eqit eq bl br) ==>
+          eq ==>
+          going (eqit eq bl br) ==>
+          eqit eq bl br) (@ITree._bind E R S).
+Proof.
+  repeat intro. subst. 
+  inv H1. gunfold H0. inv H0; simpl in *; subst; eauto.
+  - gstep. econstructor.
+  
+
+
+  subst. inv H1. gunfold H0.
+  inv H0; simpl in *; subst; eauto.
+  - gstep. econstructor. 
+    
+  intros; subst; auto.
+Qed.
+
+Lemma eqit_map {E R1 R2 S1 S2} (RR : R1 -> R2 -> Prop) bl br
       (RS : S1 -> S2 -> Prop)
       f1 f2 t1 t2 :
   (forall r1 r2, RR r1 r2 -> RS (f1 r1) (f2 r2)) ->
-  @eq_itree E _ _ RR t1 t2 ->
-  eq_itree RS (ITree.map f1 t1) (ITree.map f2 t2).
+  @eqit E _ _ RR bl br t1 t2 ->
+  eqit RS bl br (ITree.map f1 t1) (ITree.map f2 t2).
 Proof.
   unfold ITree.map; intros.
-  eapply eq_itree_bind'; eauto.
+  eapply eqit_bind'; eauto.
   intros; gstep; constructor; auto.
 Qed.
 
-Instance eq_itree_eq_map {E R S} :
+Instance eqit_eq_map {E R S} bl br :
   Proper (pointwise_relation _ eq ==>
-          eq_itree eq ==>
-          eq_itree eq) (@ITree.map E R S).
+          eqit eq bl br ==>
+          eqit eq bl br) (@ITree.map E R S).
 Proof.
-  repeat intro; eapply eq_itree_map; eauto.
+  repeat intro; eapply eqit_map; eauto.
   intros; subst; auto.
 Qed.
 
-Instance eq_itree_gcpn {E R1 R2 RS} r rg:
+Instance eqit_gcpn {E R1 R2 RS} bl br r rg:
   Proper (eq_itree eq ==> eq_itree eq ==> flip impl)
-         (gcpn2 (@eq_itree_ E R1 R2 RS) r rg).
+         (gcpn2 (@eqit_ E R1 R2 RS bl br) r rg).
 Proof.
-  repeat intro. gclo eq_itree_clo_trans. eauto.
+  repeat intro. gclo eqit_clo_trans; cycle -1.
+  - econstructor.
+    + symmetry. eauto.
+    + symmetry. eauto.
+    + eauto.
+  - firstorder.
+  - firstorder.
 Qed.
 
 Lemma bind_ret2 {E R} :
@@ -466,7 +534,7 @@ Lemma bind_ret2 {E R} :
     ITree.bind s (fun x => Ret x) ≅ s.
 Proof.
   gcofix CIH. intros.
-  rewrite !unfold_bind. gstep. repeat red.
+  rewrite !unfold_bind_. gstep. repeat red.
   genobs s os. destruct os; simpl; eauto with paco.
 Qed.
 
@@ -475,10 +543,19 @@ Lemma bind_bind {E R S T} :
     ITree.bind (ITree.bind s k) h ≅ ITree.bind s (fun r => ITree.bind (k r) h).
 Proof.
   gcofix CIH. intros.
-  unfold_eq_itree.
-  rewrite !unfold_bind.
-  gstep. repeat red. genobs s os; destruct os; simpl; eauto with paco.
-  apply Reflexive_eq_itreeF. eauto with reflexivity.
+  unfold_eqit.
+  rewrite unfold_bind_.
+  rewrite (unfold_bind_ s k).
+  rewrite unfold_bind.
+  
+  rewrite (unfold_bind s).
+  rewrite unfold_bind_.
+  assert (X:= @unfold_bind_).
+  rewrite X.
+
+  
+  gstep. repeat red. destruct (observe s); simpl; eauto with paco.
+  apply reflexivity.
 Qed.
 
 Lemma map_map {E R S T}: forall (f : R -> S) (g : S -> T) (t : itree E R),
